[WL] stronger invariants on forward subsumption
Use the normal invariants required for inprocessing. This is the last
commit on the main branch before incorporating subsumption in the WL
code and in IsaSAT.

Weidenbach_Book/Watched_Literals/Watched_Literals_List_Inprocessing.thy
@@ -3379,12 +3379,13 @@ definition forward_subsumption_all :: \<open>'v twl_st_l \<Rightarrow> 'v twl_st
        if C \<notin># dom_m (get_clauses_l S)
        then RETURN (remove1_mset C xs, S)
        else do {
-         S \<leftarrow> simplify_clause_with_unit_st C S;
-         if get_conflict_l S = None \<and> C \<in># dom_m (get_clauses_l S) \<and> length (get_clauses_l S \<propto> C) > 2 then do {
-           S \<leftarrow> try_to_forward_subsume C S;
+         T \<leftarrow> simplify_clause_with_unit_st C S;
+         ASSERT (cdcl_twl_inprocessing_l\<^sup>*\<^sup>* S T);
+         if get_conflict_l T = None \<and> C \<in># dom_m (get_clauses_l T) \<and> length (get_clauses_l T \<propto> C) > 2 then do {
+           S \<leftarrow> try_to_forward_subsume C T;
            RETURN (remove1_mset C xs, S)
          }
-         else RETURN (remove1_mset C xs, S)
+         else RETURN (remove1_mset C xs, T)
       }
     })
     (xs, S);
@@ -3538,6 +3539,7 @@ proof -
     subgoal by (rule simplify_clause_with_unit_st_pre)
       auto
     subgoal by (auto dest!: cdcl_twl_inprocessing_l.intros)
+    subgoal by auto
     subgoal by auto
     subgoal by (rule try_to_forward_subsume_pre)
     subgoal by auto
